src/HOL/Extraction/Pigeonhole.thy
@@ -245,36 +245,34 @@ code_const arbitrary_nat_pair (SML "(~1, ~1)")
 
 code_const  arbitrary_nat (SML "~1")
 
-code_module PH1
+code_module PH
 contains
   test = test
   test' = test'
   test'' = test''
 
-export_code test test' test'' in SML module_name PH2
+ML "timeit (PH.test 10)"
+ML "timeit (@{code test} 10)" 
 
-ML "timeit (PH1.test 10)"
-ML "timeit (PH2.test 10)"
+ML "timeit (PH.test' 10)"
+ML "timeit (@{code test'} 10)"
 
-ML "timeit (PH1.test' 10)"
-ML "timeit (PH2.test' 10)"
+ML "timeit (PH.test 20)"
+ML "timeit (@{code test} 20)"
 
-ML "timeit (PH1.test 20)"
-ML "timeit (PH2.test 20)"
+ML "timeit (PH.test' 20)"
+ML "timeit (@{code test'} 20)"
 
-ML "timeit (PH1.test' 20)"
-ML "timeit (PH2.test' 20)"
+ML "timeit (PH.test 25)"
+ML "timeit (@{code test} 25)"
 
-ML "timeit (PH1.test 25)"
-ML "timeit (PH2.test 25)"
+ML "timeit (PH.test' 25)"
+ML "timeit (@{code test'} 25)"
 
-ML "timeit (PH1.test' 25)"
-ML "timeit (PH2.test' 25)"
+ML "timeit (PH.test 500)"
+ML "timeit (@{code test} 500)"
 
-ML "timeit (PH1.test 500)"
-ML "timeit (PH2.test 500)"
-
-ML "timeit PH1.test''"
-ML "timeit PH2.test''"
+ML "timeit PH.test''"
+ML "timeit @{code test''}"
 
 end
